ironfleet/src/Dafny/Distributed/Protocol/RSL/FailureProof/Phase2Proof_helper1.i.dfy
@@ -3,7 +3,7 @@ include "Phase2Proof.i.dfy"
 module Rs2Phase2Proof_Helper_1 {
 import opened RslPhase2Proof_postFail_i
 
-/* WARNING: this file a timeout of 50s to verify */
+/* WARNING: this file a timeout of 60s to verify */
 
 lemma PacketsBallotInvariant_ReceiveStep(ts:TimestampedRslState, ts':TimestampedRslState, opn:OperationNumber, idx:int, tios:seq<TimestampedLIoOp<NodeIdentity, RslMessage>>) 
     requires RslAssumption(ts, opn) && RslConsistency(ts)
@@ -13,7 +13,11 @@ lemma PacketsBallotInvariant_ReceiveStep(ts:TimestampedRslState, ts':Timestamped
     requires TimestampedRslNextOneReplica(ts, ts', idx, tios);
     requires ts.t_replicas[idx].v.nextActionIndex == 0 
     ensures PacketsBallotInvariant(ts')
-{}
+{
+    forall pkt | pkt in ts'.undeliveredPackets 
+    ensures ExistingPacketsBallot(pkt)
+    {}
+}
 
 lemma PacketsBallotInvariant_NoReceiveStep(ts:TimestampedRslState, ts':TimestampedRslState, opn:OperationNumber, idx:int, tios:seq<TimestampedLIoOp<NodeIdentity, RslMessage>>) 
     requires RslAssumption(ts, opn) && RslConsistency(ts)
@@ -23,31 +27,17 @@ lemma PacketsBallotInvariant_NoReceiveStep(ts:TimestampedRslState, ts':Timestamp
     requires TimestampedRslNextOneReplica(ts, ts', idx, tios);
     requires ts.t_replicas[idx].v.nextActionIndex != 0 
     ensures PacketsBallotInvariant(ts')
-{}
-
-lemma AlwaysInvariant_Maintained(ts:TimestampedRslState, ts':TimestampedRslState, opn:OperationNumber) 
-    requires RslAssumption(ts, opn) && RslAssumption(ts', opn)
-    requires RslConsistency(ts) && RslConsistency(ts')
-    requires TimestampedRslNext(ts, ts')
-    requires RslPerfInvariant(ts, opn)
-    ensures AlwaysInvariant(ts', opn)
 {
-    assert ts'.t_replicas[1].v.replica.proposer.request_queue == [];
-    assert forall pkt | pkt in ts'.t_replicas[1].v.replica.proposer.received_1b_packets && pkt.msg.RslMessage_1b? :: forall op | op in pkt.msg.votes :: RequestBatchSrcInClientIds(ts', pkt.msg.votes[op].max_val);
-    forall pkt | pkt in ts'.undeliveredPackets && pkt.msg.v.RslMessage_2a? 
-    ensures RequestBatchSrcInClientIds(ts', pkt.msg.v.val_2a)
-    {}
-    forall pkt | pkt in ts'.undeliveredPackets && pkt.msg.v.RslMessage_2b? 
-    ensures RequestBatchSrcInClientIds(ts', pkt.msg.v.val_2b)
+    forall pkt | pkt in ts'.undeliveredPackets 
+    ensures ExistingPacketsBallot(pkt)
     {}
 }
-
 
 lemma Before2a_to_Before2b(ts:TimestampedRslState, ts':TimestampedRslState, opn:OperationNumber, tios:seq<TimestampedLIoOp<NodeIdentity, RslMessage>>) 
     requires RslAssumption(ts, opn) && RslConsistency(ts)
     requires RslAssumption(ts', opn) && RslConsistency(ts')
     requires PacketsBallotInvariant(ts) && PacketsBallotInvariant(ts')
-    requires AlwaysInvariant(ts', opn)
+    // requires AlwaysInvariant(ts', opn)
     requires TimestampedRslNext(ts, ts')
     requires !TimestampedRslNextEnvironment(ts, ts')
     requires TimestampedRslNextOneReplica(ts, ts', 1, tios);
@@ -70,13 +60,15 @@ lemma Before2a_to_Before2b(ts:TimestampedRslState, ts':TimestampedRslState, opn:
     forall pkt | pkt in ts'.t_environment.sentPackets && pkt.msg.v.RslMessage_2b?
     ensures pkt in ts.t_environment.sentPackets
     {}
+    assert forall p | p in sent_packets :: !p.msg.RslMessage_Reply?;
+    forall io | io in tios && io.LIoOpSend?
+    ensures !io.s.msg.v.RslMessage_Reply? {}
 }
 
 lemma Before2a_to_Before2a_NonLeaderAction(ts:TimestampedRslState, ts':TimestampedRslState, opn:OperationNumber, idx:int, tios:seq<TimestampedLIoOp<NodeIdentity, RslMessage>>) 
     requires RslAssumption(ts, opn) && RslConsistency(ts)
     requires RslAssumption(ts', opn) && RslConsistency(ts')
     requires PacketsBallotInvariant(ts) && PacketsBallotInvariant(ts')
-    // requires AlwaysInvariant(ts', opn)
     requires TimestampedRslNext(ts, ts')
     requires !TimestampedRslNextEnvironment(ts, ts')
     requires idx != 1;
@@ -87,9 +79,25 @@ lemma Before2a_to_Before2a_NonLeaderAction(ts:TimestampedRslState, ts':Timestamp
 {
     reveal_ExtractSentPacketsFromIos();
     reveal_UntagLIoOpSeq();
+    var ls, ls' := ts.t_replicas[idx], ts'.t_replicas[idx];
+    var nextActionIndex, nextActionIndex' := ls.v.nextActionIndex, ls'.v.nextActionIndex;
     forall pkt | pkt in ts'.t_environment.sentPackets && pkt.msg.v.RslMessage_2a?
     ensures pkt in ts.t_environment.sentPackets
-    {}
+    {
+        if pkt !in ts.t_environment.sentPackets {
+            assert ts.t_replicas[idx].v.replica.proposer.current_state == 0;
+            if nextActionIndex == 3 {
+                assert !LProposerCanNominateUsingOperationNumber(ls.v.replica.proposer, ls.v.replica.acceptor.log_truncation_point, ls.v.replica.proposer.next_operation_number_to_propose);
+                assert forall io | io in tios :: !io.LIoOpSend?;
+                assert ts.t_environment.sentPackets == ts'.t_environment.sentPackets;
+                assert false;
+            } else {
+                forall io | io in tios && io.LIoOpSend?
+                ensures !io.s.msg.v.RslMessage_2a?
+                assert false;
+            }
+        }
+    }
     forall pkt | pkt in ts'.t_environment.sentPackets && pkt.msg.v.RslMessage_2b?
     ensures BalLeq(pkt.msg.v.bal_2b, Ballot(1, 0)) && pkt.msg.v.opn_2b == opn
     {
@@ -98,6 +106,10 @@ lemma Before2a_to_Before2a_NonLeaderAction(ts:TimestampedRslState, ts':Timestamp
                 :: BalLeq(pkt.msg.v.bal_2a, Ballot(1, 0)) && pkt.msg.v.opn_2a == opn;
         }
     }
+
+    forall pkt | pkt in ts'.t_environment.sentPackets 
+    ensures !IsNew2bPacket(pkt, opn) 
+    {}
     
     forall pkt | pkt in ts'.t_environment.sentPackets
     ensures !IsNewReplyPacket(ts', pkt) 
@@ -114,7 +126,6 @@ lemma Before2b_to_Before2b_NonReceive(ts:TimestampedRslState, ts':TimestampedRsl
     requires RslAssumption(ts, opn) && RslConsistency(ts)
     requires RslAssumption(ts', opn) && RslConsistency(ts')
     requires PacketsBallotInvariant(ts) && PacketsBallotInvariant(ts')
-    // requires AlwaysInvariant(ts', opn)
     requires TimestampedRslNext(ts, ts')
     requires !TimestampedRslNextEnvironment(ts, ts')
     requires RslPerfInvariant(ts, opn)
@@ -123,21 +134,33 @@ lemma Before2b_to_Before2b_NonReceive(ts:TimestampedRslState, ts':TimestampedRsl
     requires ts.t_replicas[idx].v.nextActionIndex != 0
     ensures Before_2b_Sent_Invariant(ts', opn)
 {   
+    var ls, ls' := ts.t_replicas[idx], ts'.t_replicas[idx];
+    var nextActionIndex, nextActionIndex' := ls.v.nextActionIndex, ls'.v.nextActionIndex;
+
+
+    Before2b_to_Before2b_NonReceive_NoNewReply(ts, ts', opn, idx, tios);
     forall pkt | pkt in ts'.t_environment.sentPackets
     ensures !IsNewReplyPacket(ts', pkt) 
-    {
-        if pkt !in ts.t_environment.sentPackets {
-            assert pkt.src == ts.constants.config.replica_ids[idx];
-            assert ReplicasDistinct(ts.constants.config.replica_ids, 1, idx);
-        }
-    }
+    {}
+
     if idx != 1 {
         forall pkt | pkt in ts'.t_environment.sentPackets && pkt.msg.v.RslMessage_2a?
         ensures pkt in ts.t_environment.sentPackets
         {}
         forall pkt | pkt in ts'.t_environment.sentPackets && pkt.msg.v.RslMessage_2b?
         ensures pkt in ts.t_environment.sentPackets
-        {}
+        {
+            if pkt !in ts.t_environment.sentPackets {
+                var ios := UntagLIoOpSeq(tios);
+                var sent_packets := ExtractSentPacketsFromIos(ios);
+                assert nextActionIndex != 0;
+                assert LReplicaNoReceiveNext(ls.v.replica, nextActionIndex, ls'.v.replica, ios);
+                assert forall p | p in sent_packets :: !p.msg.RslMessage_2b?;
+                forall io | io in tios && io.LIoOpSend?
+                ensures !io.s.msg.v.RslMessage_2b? {}
+                assert false;
+            }
+        }
         assert Before_2b_Sent_Invariant(ts', opn);
     } else {
         assert ts'.t_replicas[1].v.replica.learner.unexecuted_learner_state == map[];
@@ -150,16 +173,77 @@ lemma Before2b_to_Before2b_NonReceive(ts:TimestampedRslState, ts':TimestampedRsl
         ensures pkt in ts.t_environment.sentPackets
         forall pkt | pkt in ts'.t_environment.sentPackets && pkt.msg.v.RslMessage_2b?
         ensures pkt in ts.t_environment.sentPackets
-        {}
+        {
+            if pkt !in ts.t_environment.sentPackets {
+                var ios := UntagLIoOpSeq(tios);
+                var sent_packets := ExtractSentPacketsFromIos(ios);
+                assert nextActionIndex != 0;
+                assert LReplicaNoReceiveNext(ls.v.replica, nextActionIndex, ls'.v.replica, ios);
+                assert forall p | p in sent_packets :: !p.msg.RslMessage_2b?;
+                forall io | io in tios && io.LIoOpSend?
+                ensures !io.s.msg.v.RslMessage_2b? {}
+                assert false;
+            }
+        }
         assert Before_2b_Sent_Invariant(ts', opn);
     }
 }
+
+
+lemma Before2b_to_Before2b_NonReceive_NoNewReply(ts:TimestampedRslState, ts':TimestampedRslState, opn:OperationNumber, idx:int, tios:seq<TimestampedLIoOp<NodeIdentity, RslMessage>>) 
+    requires RslAssumption(ts, opn) && RslConsistency(ts)
+    requires RslAssumption(ts', opn) && RslConsistency(ts')
+    requires PacketsBallotInvariant(ts) && PacketsBallotInvariant(ts')
+    requires TimestampedRslNext(ts, ts')
+    requires !TimestampedRslNextEnvironment(ts, ts')
+    requires RslPerfInvariant(ts, opn)
+    requires Before_2b_Sent_Invariant(ts, opn)
+    requires TimestampedRslNextOneReplica(ts, ts', idx, tios);
+    requires ts.t_replicas[idx].v.nextActionIndex != 0
+    ensures forall pkt | pkt in ts'.t_environment.sentPackets :: !IsNewReplyPacket(ts', pkt) 
+{   
+    var ls, ls' := ts.t_replicas[idx], ts'.t_replicas[idx];
+    var nextActionIndex, nextActionIndex' := ls.v.nextActionIndex, ls'.v.nextActionIndex;
+    forall pkt | pkt in ts'.t_environment.sentPackets
+    ensures !IsNewReplyPacket(ts', pkt) 
+    {
+        if IsNewReplyPacket(ts', pkt) {
+            assert pkt !in ts.t_environment.sentPackets;
+            if nextActionIndex == 6 {
+                if idx == 1 {
+                    assert ls.v.replica.executor.next_op_to_execute == OutstandingOpUnknown();
+                    var ios := UntagLIoOpSeq(tios);
+                    var sent_packets := ExtractSentPacketsFromIos(ios);
+                    assert sent_packets == [];
+                    assert forall io | io in tios :: !io.LIoOpSend?;
+                } else {
+                    assert ReplicasDistinct(ts.constants.config.replica_ids, 1, idx);
+                    forall io | io in tios && io.LIoOpSend?
+                    ensures io.s.src != ts'.constants.config.replica_ids[1] {}
+                }
+                assert false;
+            } else {
+                var ios := UntagLIoOpSeq(tios);
+                var sent_packets := ExtractSentPacketsFromIos(ios);
+                assert nextActionIndex != 0;
+                assert forall p | p in sent_packets :: !p.msg.RslMessage_Reply?;
+                forall io | io in tios && io.LIoOpSend?
+                ensures !io.s.msg.v.RslMessage_Reply? {}
+                assert false;
+            }
+        }
+    }
+}
+
+
+
+
+
 
 lemma Before2b_to_Before2b_Receive(ts:TimestampedRslState, ts':TimestampedRslState, opn:OperationNumber, idx:int, tios:seq<TimestampedLIoOp<NodeIdentity, RslMessage>>) 
     requires RslAssumption(ts, opn) && RslConsistency(ts)
     requires RslAssumption(ts', opn) && RslConsistency(ts')
     requires PacketsBallotInvariant(ts) && PacketsBallotInvariant(ts')
-    // requires AlwaysInvariant(ts', opn)
     requires TimestampedRslNext(ts, ts')
     requires !TimestampedRslNextEnvironment(ts, ts')
     requires RslPerfInvariant(ts, opn)
@@ -190,6 +274,17 @@ lemma Before2b_to_Before2b_Receive(ts:TimestampedRslState, ts':TimestampedRslSta
     forall pkt | pkt in ts'.t_environment.sentPackets && IsNewReplyPacket(ts', pkt) 
     ensures pkt in ts.t_environment.sentPackets
     {}
+
+    forall pkt | pkt in ts'.undeliveredPackets && IsNew2aPacket(pkt, opn)
+    ensures TimeLe(pkt.msg.ts, TimeBound2aDeliveryPost())
+    {
+        if pkt !in ts.undeliveredPackets {
+            forall io | io in tios && io.LIoOpSend?
+            ensures !io.s.msg.v.RslMessage_2a?
+            assert false;
+        }
+    }
+
     assert Before_2b_Sent_Invariant(ts', opn);
 }
 
