ironfleet/src/Dafny/Distributed/Protocol/RSL/FailureProof/Phase2Proof_helper2.i.dfy
@@ -3,52 +3,7 @@ include "Phase2Proof.i.dfy"
 module Rs2Phase2Proof_Helper_2 {
 import opened RslPhase2Proof_postFail_i
 
-/* WARNING: this file a timeout of 50s to verify */
-
-
-lemma Before2b_to_After2b(ts:TimestampedRslState, ts':TimestampedRslState, opn:OperationNumber, idx:int, tios:seq<TimestampedLIoOp<NodeIdentity, RslMessage>>,
-    rs:RslState, rs':RslState, iops:seq<RslIo>
-) 
-    requires rs == UntimestampRslState(ts)
-    requires rs' == UntimestampRslState(ts')
-    requires iops == UntagLIoOpSeq(tios);
-    requires RslAssumption(ts, opn) && RslConsistency(ts)
-    requires RslAssumption(ts', opn) && RslConsistency(ts')
-    requires PacketsBallotInvariant(ts) && PacketsBallotInvariant(ts')
-    requires AlwaysInvariant(ts', opn)
-    requires TimestampedRslNext(ts, ts')
-    requires !TimestampedRslNextEnvironment(ts, ts')
-    requires RslPerfInvariant(ts, opn)
-    requires Before_2b_Sent_Invariant(ts, opn)
-    requires TimestampedRslNextOneReplica(ts, ts', idx, tios);
-    requires LReplicaNextProcessPacket(rs.replicas[idx].replica, rs'.replicas[idx].replica, iops);
-    requires ts.t_replicas[idx].v.nextActionIndex == 0
-    requires |tios| > 0 && tios[0].LIoOpReceive? && tios[0].r.msg.v.RslMessage_2a? 
-    requires iops[0].r.src in rs.replicas[idx].replica.acceptor.constants.all.config.replica_ids
-    requires BalLeq(rs.replicas[idx].replica.acceptor.max_bal, iops[0].r.msg.bal_2a)
-    requires LeqUpperBound(iops[0].r.msg.opn_2a, rs.replicas[idx].replica.acceptor.constants.all.params.max_integer_val)
-    requires iops[0].r.msg.bal_2a == Ballot(1, 1)
-    ensures Before_2b_Sent_Invariant(ts', opn) || After_2b_Sent_Invariant(ts', opn)
-{
-    var r, r' := rs.replicas[idx].replica, rs'.replicas[idx].replica;
-    var m := iops[0].r.msg;
-    var sent_packets := ExtractSentPacketsFromIos(iops);
-    assert LAcceptorProcess2a(r.acceptor, r'.acceptor, iops[0].r, sent_packets);
-    var msg2b := RslMessage_2b(m.bal_2a, m.opn_2a, m.val_2a);
-    assert LBroadcastToEveryone(r.acceptor.constants.all.config, r.acceptor.constants.my_index, msg2b, sent_packets);
-    assert forall p | p in sent_packets :: LIoOpSend(p) in iops;
-    if m.opn_2a == opn {
-        var pkt_witness := sent_packets[0];
-        assert LIoOpSend(pkt_witness) in iops;
-        assert After_2b_Sent_Invariant(ts', opn);          
-    } else {
-        assert forall p | p in sent_packets && p.msg.RslMessage_2b? :: p.msg.opn_2b != opn;
-        forall pkt | pkt in ts'.t_environment.sentPackets && pkt.msg.v.RslMessage_2b?
-        ensures BalLeq(pkt.msg.v.bal_2b, Ballot(1, 1))
-        {}
-        assert Before_2b_Sent_Invariant(ts', opn);    
-    }
-}
+/* WARNING: this file a timeout of 60s to verify */
 
 
 /* Proof that a Before_2b_Sent state transitions to a Before_2b_Sent state or 
@@ -57,7 +12,6 @@ lemma Before2b_to_MaybeAfter2b_Process2a(ts:TimestampedRslState, ts':Timestamped
     requires RslAssumption(ts, opn) && RslConsistency(ts)
     requires RslAssumption(ts', opn) && RslConsistency(ts')
     requires PacketsBallotInvariant(ts) && PacketsBallotInvariant(ts')
-    requires AlwaysInvariant(ts', opn)
     requires TimestampedRslNext(ts, ts')
     requires !TimestampedRslNextEnvironment(ts, ts')
     requires TimestampedRslNextOneReplica(ts, ts', idx, tios)
@@ -116,11 +70,57 @@ lemma Before2b_to_MaybeAfter2b_Process2a(ts:TimestampedRslState, ts':Timestamped
 }
 
 
+lemma Before2b_to_After2b(ts:TimestampedRslState, ts':TimestampedRslState, opn:OperationNumber, idx:int, tios:seq<TimestampedLIoOp<NodeIdentity, RslMessage>>,
+    rs:RslState, rs':RslState, iops:seq<RslIo>
+) 
+    requires rs == UntimestampRslState(ts)
+    requires rs' == UntimestampRslState(ts')
+    requires iops == UntagLIoOpSeq(tios);
+    requires RslAssumption(ts, opn) && RslConsistency(ts)
+    requires RslAssumption(ts', opn) && RslConsistency(ts')
+    requires PacketsBallotInvariant(ts) && PacketsBallotInvariant(ts')
+    requires TimestampedRslNext(ts, ts')
+    requires !TimestampedRslNextEnvironment(ts, ts')
+    requires RslPerfInvariant(ts, opn)
+    requires Before_2b_Sent_Invariant(ts, opn)
+    requires TimestampedRslNextOneReplica(ts, ts', idx, tios);
+    requires LReplicaNextProcessPacket(rs.replicas[idx].replica, rs'.replicas[idx].replica, iops);
+    requires ts.t_replicas[idx].v.nextActionIndex == 0
+    requires |tios| > 0 && tios[0].LIoOpReceive? && tios[0].r.msg.v.RslMessage_2a? 
+    requires iops[0].r.src in rs.replicas[idx].replica.acceptor.constants.all.config.replica_ids
+    requires BalLeq(rs.replicas[idx].replica.acceptor.max_bal, iops[0].r.msg.bal_2a)
+    requires LeqUpperBound(iops[0].r.msg.opn_2a, rs.replicas[idx].replica.acceptor.constants.all.params.max_integer_val)
+    requires iops[0].r.msg.bal_2a == Ballot(1, 1)
+    ensures Before_2b_Sent_Invariant(ts', opn) || After_2b_Sent_Invariant(ts', opn)
+{
+    var m := iops[0].r.msg;
+    var sent_packets := ExtractSentPacketsFromIos(iops);
+    assert LAcceptorProcess2a(rs.replicas[idx].replica.acceptor, rs'.replicas[idx].replica.acceptor, iops[0].r, sent_packets);
+    var msg2b := RslMessage_2b(m.bal_2a, m.opn_2a, m.val_2a);
+    assert LBroadcastToEveryone(rs.replicas[idx].replica.acceptor.constants.all.config, rs.replicas[idx].replica.acceptor.constants.my_index, msg2b, sent_packets);
+    assert forall p | p in sent_packets :: LIoOpSend(p) in iops;
+    if m.opn_2a == opn {
+        var pkt_witness := sent_packets[0];
+        reveal_ExtractSentPacketsFromIos();
+        reveal_UntagLIoOpSeq();
+        assert forall p | p in sent_packets :: !p.msg.RslMessage_Reply?;
+        assert LIoOpSend(pkt_witness) in iops;
+        assert After_2b_Sent_Invariant(ts', opn);          
+    } else {
+        assert forall p | p in sent_packets && p.msg.RslMessage_2b? :: p.msg.opn_2b != opn;
+        forall pkt | pkt in ts'.t_environment.sentPackets && pkt.msg.v.RslMessage_2b?
+        ensures BalLeq(pkt.msg.v.bal_2b, Ballot(1, 1))
+        {}
+        assert Before_2b_Sent_Invariant(ts', opn);    
+    }
+}
+
+
+
 lemma After2b_to_After2b_NonLeaderAction(ts:TimestampedRslState, ts':TimestampedRslState, opn:OperationNumber, idx:int, tios:seq<TimestampedLIoOp<NodeIdentity, RslMessage>>) 
     requires RslAssumption(ts, opn) && RslConsistency(ts)
     requires RslAssumption(ts', opn) && RslConsistency(ts')
     requires PacketsBallotInvariant(ts) && PacketsBallotInvariant(ts')
-    requires AlwaysInvariant(ts', opn)
     requires TimestampedRslNext(ts, ts')
     requires !TimestampedRslNextEnvironment(ts, ts')
     requires TimestampedRslNextOneReplica(ts, ts', idx, tios)
@@ -130,7 +130,7 @@ lemma After2b_to_After2b_NonLeaderAction(ts:TimestampedRslState, ts':Timestamped
     ensures After_2b_Sent_Invariant(ts', opn)
 {
     assert ts'.t_replicas[1] == ts.t_replicas[1];
-    After2b_to_After2b_NonLeaderAction_2bBalOpn(ts, ts', opn, idx, tios);
+    After2b_to_After2b_2bBalOpn(ts, ts', opn, idx, tios);
 
     forall p | p in ts'.undeliveredPackets && IsNew2aPacket(p, opn)
     ensures p in ts.undeliveredPackets {
@@ -155,16 +155,14 @@ lemma After2b_to_After2b_NonLeaderAction(ts:TimestampedRslState, ts':Timestamped
 }
 
 
-lemma After2b_to_After2b_NonLeaderAction_2bBalOpn(ts:TimestampedRslState, ts':TimestampedRslState, opn:OperationNumber, idx:int, tios:seq<TimestampedLIoOp<NodeIdentity, RslMessage>>) 
+lemma After2b_to_After2b_2bBalOpn(ts:TimestampedRslState, ts':TimestampedRslState, opn:OperationNumber, idx:int, tios:seq<TimestampedLIoOp<NodeIdentity, RslMessage>>) 
     requires RslAssumption(ts, opn) && RslConsistency(ts)
     requires RslAssumption(ts', opn) && RslConsistency(ts')
     requires PacketsBallotInvariant(ts) && PacketsBallotInvariant(ts')
-    requires AlwaysInvariant(ts', opn)
     requires TimestampedRslNext(ts, ts')
     requires !TimestampedRslNextEnvironment(ts, ts')
     requires TimestampedRslNextOneReplica(ts, ts', idx, tios)
     requires RslPerfInvariant(ts, opn)
-    requires idx != 1;
     requires After_2b_Sent_Invariant(ts, opn)
     ensures forall pkt | pkt in ts'.t_environment.sentPackets && pkt.msg.v.RslMessage_2b? :: BalLeq(pkt.msg.v.bal_2b, Ballot(1, 1)) && pkt.msg.v.opn_2b == opn
 {
@@ -173,13 +171,12 @@ lemma After2b_to_After2b_NonLeaderAction_2bBalOpn(ts:TimestampedRslState, ts':Ti
     ensures BalLeq(pkt.msg.v.bal_2b, Ballot(1, 1)) && pkt.msg.v.opn_2b == opn
     {
         var sr, sr', ios := UntimestampRslState(ts), UntimestampRslState(ts'), UntagLIoOpSeq(tios);
-        var r, r' := sr.replicas[idx].replica, sr'.replicas[idx].replica;
         if sr.replicas[idx].nextActionIndex == 0 {
             var msg := tios[0].r.msg;
             if msg.v.RslMessage_2a? {
-                if tios[0].r.src in r.acceptor.constants.all.config.replica_ids
-                    && BalLeq(r.acceptor.max_bal, msg.v.bal_2a)
-                    && LeqUpperBound(msg.v.opn_2a, r.acceptor.constants.all.params.max_integer_val)
+                if tios[0].r.src in sr.replicas[idx].replica.acceptor.constants.all.config.replica_ids
+                    && BalLeq(sr.replicas[idx].replica.acceptor.max_bal, msg.v.bal_2a)
+                    && LeqUpperBound(msg.v.opn_2a, sr.replicas[idx].replica.acceptor.constants.all.params.max_integer_val)
                 {
                     var sent_packets := ExtractSentPacketsFromIos(ios);
                     forall sp | sp in sent_packets 
@@ -206,5 +203,231 @@ lemma After2b_to_After2b_NonLeaderAction_2bBalOpn(ts:TimestampedRslState, ts':Ti
         }
     }
 }
+
+
+lemma After2b_to_After2b_LeaderAction(ts:TimestampedRslState, ts':TimestampedRslState, opn:OperationNumber, idx:int, tios:seq<TimestampedLIoOp<NodeIdentity, RslMessage>>) 
+    requires RslAssumption(ts, opn) && RslConsistency(ts)
+    requires RslAssumption(ts', opn) && RslConsistency(ts')
+    requires PacketsBallotInvariant(ts) && PacketsBallotInvariant(ts')
+    requires TimestampedRslNext(ts, ts')
+    requires !TimestampedRslNextEnvironment(ts, ts')
+    requires TimestampedRslNextOneReplica(ts, ts', idx, tios)
+    requires RslPerfInvariant(ts, opn)
+    requires idx == 1;
+    requires After_2b_Sent_Invariant(ts, opn)
+    ensures After_2b_Sent_Invariant(ts', opn)
+{
+    var lr, lr' := ts.t_replicas[1].v.replica, ts'.t_replicas[1].v.replica;
+    var nextActionIndex, nextActionIndex' := ts.t_replicas[1].v.nextActionIndex, ts'.t_replicas[1].v.nextActionIndex;
+
+    After2b_to_After2b_2bBalOpn(ts, ts', opn, idx, tios);
+    assert All2aPackets_BalLeq_Opn(ts', Ballot(1, 1), opn);
+    assert All2bPackets_BalLeq_Opn(ts', Ballot(1, 1), opn);
+    assert PerformanceGuarantee_2a(ts', opn); 
+
+    After2b_to_After2b_LeaderAction_TimeBound2b(ts, ts', opn, tios);
+    forall p | p in ts'.undeliveredPackets && IsNew2bPacket(p, opn)
+    ensures TimeLe(p.msg.ts, TimeBound2bDeliveryPost())
+    {}
+
+    forall p | p in ts'.undeliveredPackets && IsNewReplyPacket(ts', p)
+    ensures TimeLe(p.msg.ts, TimeBoundReplyFailure())
+    {}
+
+
+    After2b_to_After2b_LeaderAction_PreExecution(ts, ts', opn, tios);
+
+    After2b_to_After2b_LeaderAction_PostExecution(ts, ts', opn, tios);
+
+    After2b_to_After2b_LeaderAction_LearnedBatchNotEmpty(ts, ts', opn, tios);
+
+    forall opn' | opn' in lr'.learner.unexecuted_learner_state 
+    ensures opn' == opn && |lr'.learner.unexecuted_learner_state[opn'].received_2b_message_senders| > 0
+    {}
+}
+
+
+lemma After2b_to_After2b_LeaderAction_TimeBound2b(ts:TimestampedRslState, ts':TimestampedRslState, opn:OperationNumber, tios:seq<TimestampedLIoOp<NodeIdentity, RslMessage>>) 
+    requires RslAssumption(ts, opn) && RslConsistency(ts)
+    requires RslAssumption(ts', opn) && RslConsistency(ts')
+    requires PacketsBallotInvariant(ts) && PacketsBallotInvariant(ts')
+    requires TimestampedRslNext(ts, ts')
+    requires !TimestampedRslNextEnvironment(ts, ts')
+    requires TimestampedRslNextOneReplica(ts, ts', 1, tios)
+    requires RslPerfInvariant(ts, opn)
+    requires After_2b_Sent_Invariant(ts, opn)
+    requires All2aPackets_BalLeq_Opn(ts, Ballot(1, 1), opn)
+    requires All2bPackets_BalLeq_Opn(ts, Ballot(1, 1), opn)
+    requires PerformanceGuarantee_2a(ts, opn)
+    requires PerformanceGuarantee_2b(ts, opn)
+    requires PerformanceGuarantee_Response(ts)
+    ensures forall p | p in ts'.undeliveredPackets && IsNew2bPacket(p, opn) :: TimeLe(p.msg.ts, TimeBound2bDeliveryPost())
+{
+    var ls, ls' := ts.t_replicas[1], ts'.t_replicas[1];
+    var nextActionIndex, nextActionIndex' := ls.v.nextActionIndex, ls'.v.nextActionIndex;
+    forall p | p in ts'.undeliveredPackets && IsNew2bPacket(p, opn) 
+    ensures TimeLe(p.msg.ts, TimeBound2bDeliveryPost())
+    {
+        if p !in ts.undeliveredPackets {
+            if nextActionIndex == 0 {
+                assert TimeLe(p.msg.ts, TimeBound2bDeliveryPost());
+            } else {
+                forall io | io in tios && io.LIoOpSend?
+                ensures !io.s.msg.v.RslMessage_2b? {}
+                assert false;
+            }
+        }
+    }
+}
+
+
+lemma After2b_to_After2b_LeaderAction_LearnedBatchNotEmpty(ts:TimestampedRslState, ts':TimestampedRslState, opn:OperationNumber, tios:seq<TimestampedLIoOp<NodeIdentity, RslMessage>>) 
+    requires RslAssumption(ts, opn) && RslConsistency(ts)
+    requires RslAssumption(ts', opn) && RslConsistency(ts')
+    requires PacketsBallotInvariant(ts) && PacketsBallotInvariant(ts')
+    requires TimestampedRslNext(ts, ts')
+    requires !TimestampedRslNextEnvironment(ts, ts')
+    requires TimestampedRslNextOneReplica(ts, ts', 1, tios)
+    requires RslPerfInvariant(ts, opn)
+    requires After_2b_Sent_Invariant(ts, opn)
+    requires All2aPackets_BalLeq_Opn(ts, Ballot(1, 1), opn)
+    requires All2bPackets_BalLeq_Opn(ts, Ballot(1, 1), opn)
+    requires PerformanceGuarantee_2a(ts, opn)
+    requires PerformanceGuarantee_2b(ts, opn)
+    requires PerformanceGuarantee_Response(ts)
+    ensures Get2bCount(ts'.t_replicas[1].v.replica, opn, Ballot(1, 1)) > 0 ==>|ts'.t_replicas[1].v.replica.learner.unexecuted_learner_state[opn].candidate_learned_value| >= 1
+{
+    var ls, ls' := ts.t_replicas[1], ts'.t_replicas[1];
+    var nextActionIndex, nextActionIndex' := ls.v.nextActionIndex, ls'.v.nextActionIndex;
+    if Get2bCount(ls.v.replica, opn, Ballot(1, 1)) == 0 {
+        if nextActionIndex == 0 && tios[0].r.msg.v.RslMessage_2b?{
+            var op_learnable := ls.v.replica.executor.ops_complete < opn || (ls.v.replica.executor.ops_complete == opn && ls.v.replica.executor.next_op_to_execute.OutstandingOpUnknown?);
+            var m := tios[0].r.msg;
+            if op_learnable {
+                if tios[0].r.src !in ls.v.replica.learner.constants.all.config.replica_ids || BalLt(m.v.bal_2b, ls.v.replica.learner.max_ballot_seen) {
+                    assert Get2bCount(ls'.v.replica, opn, Ballot(1, 1)) == 0;
+                } else if BalLt(ls.v.replica.learner.max_ballot_seen, m.v.bal_2b) {
+                    assert |m.v.val_2b| > 0;
+                    assert ls'.v.replica.learner.unexecuted_learner_state[opn].candidate_learned_value == m.v.val_2b;
+                } else if opn !in ls.v.replica.learner.unexecuted_learner_state {
+                    assert |m.v.val_2b| > 0;
+                    assert ls'.v.replica.learner.unexecuted_learner_state[opn].candidate_learned_value == m.v.val_2b;
+                }
+                else if tios[0].r.src in ls.v.replica.learner.unexecuted_learner_state[opn].received_2b_message_senders {
+                    assert Get2bCount(ls'.v.replica, opn, Ballot(1, 1)) == 0;
+                } else {
+                    assert false;
+                }
+                assert |ls'.v.replica.learner.unexecuted_learner_state[opn].candidate_learned_value| >= 1;
+            } else {
+                assert Get2bCount(ls'.v.replica, opn, Ballot(1, 1)) == 0;
+            }
+        } else {
+            assert Get2bCount(ls'.v.replica, opn, Ballot(1, 1)) == 0;
+        }
+    }
+}
+
+
+lemma After2b_to_After2b_LeaderAction_PostExecution(ts:TimestampedRslState, ts':TimestampedRslState, opn:OperationNumber, tios:seq<TimestampedLIoOp<NodeIdentity, RslMessage>>) 
+    requires RslAssumption(ts, opn) && RslConsistency(ts)
+    requires RslAssumption(ts', opn) && RslConsistency(ts')
+    requires PacketsBallotInvariant(ts) && PacketsBallotInvariant(ts')
+    requires TimestampedRslNext(ts, ts')
+    requires !TimestampedRslNextEnvironment(ts, ts')
+    requires TimestampedRslNextOneReplica(ts, ts', 1, tios)
+    requires RslPerfInvariant(ts, opn)
+    requires After_2b_Sent_Invariant(ts, opn)
+    requires All2aPackets_BalLeq_Opn(ts, Ballot(1, 1), opn)
+    requires All2bPackets_BalLeq_Opn(ts, Ballot(1, 1), opn)
+    requires PerformanceGuarantee_2a(ts, opn)
+    requires PerformanceGuarantee_2b(ts, opn)
+    requires PerformanceGuarantee_Response(ts)
+    ensures ts'.t_replicas[1].v.replica.executor.ops_complete > opn ==> After_Request_Executed(ts', ts'.t_replicas[1], opn)
+{
+    var ls, ls' := ts.t_replicas[1], ts'.t_replicas[1];
+    var nextActionIndex, nextActionIndex' := ls.v.nextActionIndex, ls'.v.nextActionIndex;
+    if ls'.v.replica.executor.ops_complete > opn {     
+        if ls.v.replica.executor.ops_complete == opn {
+            if nextActionIndex == 6 {
+                var ios := UntagLIoOpSeq(tios);
+                var sent_packets := ExtractSentPacketsFromIos(ios);
+                assert ls.v.replica.executor.next_op_to_execute.OutstandingOpKnown?;
+                reveal_ExtractSentPacketsFromIos();
+                reveal_UntagLIoOpSeq();
+                assert After_Request_Executed(ts', ts'.t_replicas[1], opn);
+            } else {
+                assert ls'.v.replica.executor.ops_complete == opn;
+                assert false;
+            }
+        }
+       assert  After_Request_Executed(ts', ts'.t_replicas[1], opn);
+    }
+}
+
+
+lemma After2b_to_After2b_LeaderAction_PreExecution(ts:TimestampedRslState, ts':TimestampedRslState, opn:OperationNumber, tios:seq<TimestampedLIoOp<NodeIdentity, RslMessage>>) 
+    requires RslAssumption(ts, opn) && RslConsistency(ts)
+    requires RslAssumption(ts', opn) && RslConsistency(ts')
+    requires PacketsBallotInvariant(ts) && PacketsBallotInvariant(ts')
+    requires TimestampedRslNext(ts, ts')
+    requires !TimestampedRslNextEnvironment(ts, ts')
+    requires TimestampedRslNextOneReplica(ts, ts', 1, tios)
+    requires RslPerfInvariant(ts, opn)
+    requires After_2b_Sent_Invariant(ts, opn)
+    requires All2aPackets_BalLeq_Opn(ts, Ballot(1, 1), opn)
+    requires All2bPackets_BalLeq_Opn(ts, Ballot(1, 1), opn)
+    requires PerformanceGuarantee_2a(ts, opn)
+    requires PerformanceGuarantee_2b(ts, opn)
+    requires PerformanceGuarantee_Response(ts)
+    ensures ts'.t_replicas[1].v.replica.executor.ops_complete == opn ==> Before_Request_Executed(ts', ts'.t_replicas[1], opn)
+{
+    var ls, ls' := ts.t_replicas[1], ts'.t_replicas[1];
+    var nextActionIndex, nextActionIndex' := ls.v.nextActionIndex, ls'.v.nextActionIndex;
+
+    if ls'.v.replica.executor.ops_complete == opn {      
+        if Get2bCount(ls.v.replica, opn, Ballot(1, 1)) < LMinQuorumSize(ts.constants.config) {
+            if nextActionIndex == 0 {
+                if tios[0].r.msg.v.RslMessage_2b? && tios[0].r.msg.v.opn_2b == opn {
+                    var pkt := tios[0].r;
+                    assert nextActionIndex == 0 && nextActionIndex' == 1;
+                    assert pkt.msg.v.bal_2b == Ballot(1, 1);
+                    assert pkt in ts.undeliveredPackets;
+                    assert IsNew2bPacket(pkt, opn);
+                    assert TimeLe(pkt.msg.ts, TimeBound2bDeliveryPost());
+                    assert ts.t_environment.nextStep.nodeStep == RslStep(0);
+                    assert TimeLe(TimeMax(pkt.msg.ts, ls.ts), pkt.msg.ts + MaxQueueTime);
+                    assert TimeLe(ls'.ts, pkt.msg.ts + MaxQueueTime + StepToTimeDelta(RslStep(0)));
+                    assert TimeLe(ls'.ts, TimeBound2bDeliveryPost() + MaxQueueTime + TimeActionRange(1));
+                    assert TimeLe(ls'.ts, TimeBoundPhase2LeaderPost(nextActionIndex'));
+                } else {
+                    assert Get2bCount(ls'.v.replica, opn, Ballot(1, 1)) <= Get2bCount(ls.v.replica, opn, Ballot(1, 1));
+                }
+            } else {
+                assert Get2bCount(ls'.v.replica, opn, Ballot(1, 1)) <= Get2bCount(ls.v.replica, opn, Ballot(1, 1));
+            }
+        } else if Get2bCount(ls.v.replica, opn, Ballot(1, 1)) == LMinQuorumSize(ts.constants.config) {
+            if nextActionIndex == 0 || nextActionIndex > 6{
+                assert exists pkt :: pkt in ts'.t_environment.sentPackets && IsNewReplyPacket(ts', pkt);
+                assert false;
+            } else {
+                if |tios| > 0 && tios[0].LIoOpReceive? {
+                    assert false;
+                } else if |tios| > 0 && tios[0].LIoOpTimeoutReceive? {
+                    assert false;
+                } else {
+                    assert TimestampedRslNextOneReplica(ts, ts', 1, tios);
+                    var hstep := ts.t_environment.nextStep.nodeStep;
+                    assert hstep == RslStep(nextActionIndex);
+                    assert nextActionIndex' == nextActionIndex + 1;
+                    assert TimeLe(ls'.ts, TimeBoundPhase2LeaderPost(nextActionIndex'));
+                }
+            }
+        } 
+    }   
+}
+
+
+
 
 }
